README.md
@@ -4,6 +4,9 @@ HEEEEEEEELLO!
 
 Date: Aug 26
 Next steps:
-1. Actually read LessThanInv to make sure it works
+~~1. Actually read LessThanInv to make sure it works~~
 2. Prove Cycle.lean (Deps can be reused)
 3. Prove EndsInFixPoint (maybe I should try this before 2, I'm so tired of these Deps, honestly)
+
+Date: Sept 18
+Looked at LessThanInv. It makes sense.
